theory/JITSimple.thy
@@ -1,8 +1,0 @@
-theory JITSimple
-imports
-  Main
-  rBPFCommType rBPFSyntax
-  JITCommType x86 vm
-begin
-
-end
