theory/x64DecodeProof1.thy
@@ -10,10 +10,55 @@ lemma list_nth_right: "v = l!n \<Longrightarrow> l!n = v" using HOL.sym by simp
 lemma if_false_eq: "a \<noteq> b \<Longrightarrow> (if a = b then c else d) = d" using HOL.if_not_P
   by argo 
 
-lemma construct_rex_to_u8_neq_144: "construct_rex_to_u8 b0 b1 b2 b3 \<noteq> 144"
+lemma construct_rex_to_u8_eq_64:
+  " construct_rex_to_u8 b0 b1 b2 b3 = 64 \<Longrightarrow>
+      b0 = False \<and> b1 = False \<and> b2 = False \<and> b3 = False"
   apply (unfold construct_rex_to_u8_def bitfield_insert_u8_def Let_def u8_of_bool_def)
   apply (cases b0; cases b1; cases b2; cases b3; simp)
   done
+
+lemma construct_rex_to_u8_neq_64:
+  "construct_rex_to_u8 b0 b1 b2 b3 \<noteq> 64 \<Longrightarrow>
+    bitfield_extract_u8 0 4 (construct_rex_to_u8 b0 b1 b2 b3) \<noteq> 0"
+  apply (unfold construct_rex_to_u8_def bitfield_insert_u8_def bitfield_extract_u8_def Let_def u8_of_bool_def)
+  apply (cases b0; cases b1; cases b2; cases b3; simp)
+  done
+
+lemma construct_rex_to_u8_neq_64_1:
+  "construct_rex_to_u8 b0 b1 b2 b3 \<noteq> 64 \<Longrightarrow>
+    b0 = True \<or> b1 = True \<or> b2 = True \<or> b3 = True"
+  apply (unfold construct_rex_to_u8_def bitfield_insert_u8_def bitfield_extract_u8_def Let_def u8_of_bool_def)
+  apply (cases b0; cases b1; cases b2; cases b3; simp)
+  done
+
+lemma construct_rex_to_u8_range:
+  "0x40 \<le> construct_rex_to_u8 b0 b1 b2 b3 \<and> construct_rex_to_u8 b0 b1 b2 b3 \<le> 0x4f"
+  apply (unfold construct_rex_to_u8_def bitfield_insert_u8_def Let_def u8_of_bool_def)
+  apply (cases b0; cases b1; cases b2; cases b3; simp)
+  done
+
+lemma construct_rex_to_u8_range_outside [simp]:
+  "v < 0x40 \<or> v > 0x4f \<Longrightarrow> construct_rex_to_u8 b0 b1 b2 b3 \<noteq> v"
+  using construct_rex_to_u8_range
+  using linorder_not_less by blast
+
+lemma bitfield_extract_u8_construct_rex_to_u8_4 [simp]:
+  " v = construct_rex_to_u8 b0 b1 b2 b3 \<Longrightarrow>
+    bitfield_extract_u8 4 4 v = 4"
+  apply (unfold construct_rex_to_u8_def, simp add: bitfield_simps)
+  apply (simp add: bitfield_extract_u8_def)
+  done
+
+lemma ireg_of_u8_bitfield_extract_u8_u8_of_ireg_same [bitfield_simps]:
+  "ireg_of_u8 (bitfield_extract_u8 0 4 (u8_of_ireg r)) = Some r"
+  by (cases r; simp add: bitfield_extract_u8_def ireg_of_u8_def)
+
+lemma nat_3_plus_1: "3 + 1 = (4::nat)" by simp
+
+lemma ireg_of_u8_extract_3_some [bitfield_simps]:
+  " (bitfield_extract_u8 3 1 (u8_of_ireg r) \<noteq> 0) = False \<Longrightarrow>
+      ireg_of_u8 (bitfield_extract_u8 0 3 (u8_of_ireg r)) = Some r"
+  by (cases r; simp add: bitfield_extract_u8_def ireg_of_u8_def)
 
 lemma x64_encode_decode_consistency:
   "list_in_list l_bin pc l \<Longrightarrow> Some l_bin = x64_encode ins \<Longrightarrow>
@@ -23,10 +68,61 @@ lemma x64_encode_decode_consistency:
   subgoal for rd rs
     apply (simp add: split: if_split_asm; erule conjE)
     subgoal
+      apply (drule construct_rex_to_u8_eq_64; erule conjE; erule conjE; erule conjE)
       apply (drule HOL.sym [of _ "l ! Suc pc"])
-      apply (simp add: x64_decode_def
-          bitfield_extract_u8_def bitfield_insert_u8_def ireg_of_u8_def)
-      apply (simp add: Let_def)
+      apply (simp only: x64_decode_def Let_def)
+      apply (subst if_not_P, simp)
+      apply (subst if_not_P, simp)
+      apply (subst if_not_P, simp)
+      apply (subst if_not_P [of "137 = 102"], simp)
+      apply (subst if_P [of "bitfield_extract_u8 4 4 137 \<noteq> 4"], simp add: bitfield_extract_u8_def)
+      apply (subst if_not_P [of "bitfield_extract_u8 3 5 137 = 10"], simp add: bitfield_extract_u8_def)
+      apply (subst if_not_P [of "bitfield_extract_u8 3 5 137 = 11"], simp add: bitfield_extract_u8_def)
+      apply (subst if_not_P [of "137 = 15"], simp)
+      apply (subst if_not_P, simp)
+      apply (subst if_not_P, simp)
+      apply (subst if_P [of "137 = 137"], simp)
+      apply (simp only: Nat.One_nat_def[symmetric])
+      apply (simp only: Nat.Suc_eq_plus1 construct_modsib_to_u8_def bitfield_simps)
+      apply (subst if_P [of "bitfield_extract_u8 0 2 3 = 3"], simp add: bitfield_extract_u8_def)
+      apply (simp add: case_optionE bitfield_simps)
+      done
+    subgoal
+      apply (erule conjE)
+      apply (drule HOL.sym [of _ "l ! Suc (Suc pc)"])
+      apply (simp only: x64_decode_def Let_def)
+      apply (subst if_not_P [of "l ! pc = 144"], drule HOL.sym [of _ "l ! pc"], simp)
+      apply (subst if_not_P [of "l ! pc = 153"], drule HOL.sym [of _ "l ! pc"], simp)
+      apply (subst if_not_P [of "l ! pc = 195"], drule HOL.sym [of _ "l ! pc"], simp)
+      apply (subst if_not_P [of "l ! pc = 102"], drule HOL.sym [of _ "l ! pc"], simp)
+      apply (subst if_not_P [of "l ! pc = 15"], drule HOL.sym [of _ "l ! pc"], simp)
+      apply (subst if_not_P [of "bitfield_extract_u8 4 4 (l ! pc) \<noteq> 4"], drule HOL.sym [of _ "l ! pc"], simp)
+      apply (subst if_not_P [of "bitfield_extract_u8 0 4 (l ! pc) = 0"], metis construct_rex_to_u8_neq_64)
+      apply (subst if_not_P [of "l ! (pc + 1) = 153"], simp)
+      apply (subst if_not_P [of "bitfield_extract_u8 3 5 (l ! (pc + 1)) = 10"], simp add: bitfield_extract_u8_def)
+      apply (subst if_not_P [of "bitfield_extract_u8 3 5 (l ! (pc + 1)) = 11"], simp add: bitfield_extract_u8_def)
+      apply (subst if_not_P [of "bitfield_extract_u8 3 5 (l ! (pc + 1)) = 23"], simp add: bitfield_extract_u8_def)
+      apply (subst if_not_P [of "l ! (pc + 1) = 104"], simp)
+      apply (subst if_not_P [of "l ! (pc + 1) = 15"], simp)
+      apply (subst if_P [of "l ! (pc + 1) = 137"], simp)
+      apply (simp only: construct_modsib_to_u8_def)
+      apply (subst if_P [of "bitfield_extract_u8 6 2 (l ! (pc + 2)) = 3"], simp add: bitfield_simps, simp add: bitfield_extract_u8_def)
+      apply (drule HOL.sym [of _ "l ! pc"])
+      apply (insert construct_rex_to_u8_neq_64_1)
+      apply (simp only: construct_rex_to_u8_def Num.add_2_eq_Suc'[symmetric] bitfield_simps nat_3_plus_1)
+      apply (subst if_not_P, simp)
+      apply (subst if_P [of "bitfield_extract_u8 0 1 (u8_of_bool False) = 0 \<and> bitfield_extract_u8 0 1 (u8_of_bool False) = 0"], simp add: bitfield_extract_u8_def u8_of_bool_def)
+      apply (subst if_not_P [of "bitfield_extract_u8 3 1 (u8_of_ireg rs) = 0 \<and> bitfield_extract_u8 3 1 (u8_of_ireg rd) = 0"], simp)
+      apply (metis u8_of_bool_false)
+      apply (simp add: case_optionE)
+      done
+    done
+
+
+      value "bitfield_extract_u8 0 1 (u8_of_bool False) = 0 \<and> bitfield_extract_u8 0 1 (u8_of_bool False) = 0"
+      find_theorems "Suc (Suc ?a)"
+      value "bitfield_extract_u8 0 2 3 = 3"
+
 (*
     apply (cases ins; simp add: Let_def construct_rex_to_u8_neq_144) *)
 (*
