theory/x86CommType.thy
@@ -54,7 +54,7 @@ x86_sib_scale :: u8
 x86_sib_index :: u8
 x86_sib_base  :: u8
 
-definition construct_rex_to_u8 :: "bool\<Rightarrow> bool \<Rightarrow> bool \<Rightarrow> bool \<Rightarrow>u8" where
+definition construct_rex_to_u8 :: "bool \<Rightarrow> bool \<Rightarrow> bool \<Rightarrow> bool \<Rightarrow> u8" where
 "construct_rex_to_u8 w r x b =
    bitfield_insert_u8 4 4 
     (bitfield_insert_u8 3 1
